---
tags:
  - category/note
  - status/finished
  - topic/analisi-I
date: 27-10-2023 18:33:51
links:
  - "[[Lecture 27102023135003]]"
---
# Algebra delle derivate
---
## Introduzione
### Elementari
$$(f \pm g)'(x_{0}) = f'(x_{0}) \pm g'(x_{0})$$

$$(f \cdot g)'(x_{0}) = f'(x_{0}) \cdot g(x_{0}) + f(x_{0}) \cdot g'(x_{0})$$
dimostrazione perch√© $(f \cdot g)'(x_{0}) \neq f'(x_{0}) \cdot g'(c_{0})$.

$$(\frac{f}{h})'(x_{0}) = \frac{f'(x_{0}) \cdot g(x_{0}) - f(x_{0}) \cdot g'(x_{0})}{g^{2}(x_{0})}$$

### Ricavate
$$(\frac{1}{f})'(x_{0}) = -\frac{Df(x_{0})}{f^{2}(x_{0})}$$

### Funzioni composte
Anche detta **regola della catena**:
$$(f \circ g)'(x_{0}) = f'(g(x_{0})) \cdot g'(x_{0})$$

## Referenze